intermediate/Veritas.Intermediate.Blum.fsti
@@ -1,0 +1,90 @@
+module Veritas.Intermediate.Blum
+
+open FStar.Seq
+open Veritas.Key
+open Veritas.MultiSet
+open Veritas.MultiSetHash
+open Veritas.Intermediate.Global
+open Veritas.Intermediate.Logs
+open Veritas.Intermediate.TSLog
+open Veritas.Intermediate.Thread
+open Veritas.Intermediate.VerifierConfig
+
+module I = Veritas.Interleave
+module SpecB = Veritas.Verifier.Blum
+module IntG = Veritas.Intermediate.Global
+module IntT = Veritas.Intermediate.Thread
+
+(* sequence of blum adds in the time sequenced log *)
+val add_seq (#vcfg:_) (ils: its_log vcfg): seq ms_hashfn_dom
+
+(* the addset in a time sequenced log *)
+let add_set #vcfg (ils: its_log vcfg): mset_ms_hashfn_dom 
+  = seq2mset #_ #ms_hashfn_dom_cmp (add_seq ils)
+
+let blum_add_elem (#vcfg:_) (itsl: its_log vcfg) (i: I.seq_index itsl {is_blum_add (I.index itsl i)}) = 
+  IntT.blum_add_elem (I.index itsl i)
+  
+val lemma_add_elem_correct (#vcfg:_) (itsl: its_log vcfg) (i: I.seq_index itsl):
+  Lemma (requires (is_blum_add (I.index itsl i)))
+        (ensures (add_set itsl `contains` blum_add_elem itsl i))
+        [SMTPat (I.index itsl i)]
+
+(* sequence of blum adds restricted to key k *)
+val add_seq_key (#vcfg:_) (itsl: its_log vcfg) (k:key): seq ms_hashfn_dom
+
+(* the addset restricted to key k *)
+let add_set_key (#vcfg:_) (itsl: its_log vcfg) (k:key): mset_ms_hashfn_dom
+  = seq2mset #_ #ms_hashfn_dom_cmp (add_seq_key itsl k)
+
+(* the blum adds in the time sequenced log should be the same as global add set *)
+val lemma_add_set_correct (#vcfg:_) (itsl: its_log vcfg): 
+  Lemma (ensures (add_set itsl == IntG.add_set (g_logS_of itsl)))
+
+(* if the tail element is a blum add, then the add set is obtained by adding that 
+ * blum add to the prefix *)
+val lemma_add_set_key_extend  (#vcfg:_) (itsl: its_log vcfg {I.length itsl > 0}):
+  Lemma (requires (is_blum_add (I.telem itsl)))
+        (ensures (let i = I.length itsl - 1 in
+                  let e = I.index itsl i in
+                  let be = blum_add_elem itsl i in
+                  let k = key_of be in
+                  let itsl' = I.prefix itsl i in
+                  add_set_key itsl k == 
+                  add_elem (add_set_key itsl' k) be))
+
+val some_add_elem_idx (#vcfg:_) (itsl: its_log vcfg) 
+  (be: ms_hashfn_dom{add_set itsl `contains` be}): 
+  (i:(I.seq_index itsl){is_blum_add (I.index itsl i) /\
+                        be = blum_add_elem itsl i})
+
+val lemma_add_set_key_contains_only (#vcfg:_) (itsl: its_log vcfg) (k:key) (be: ms_hashfn_dom):
+  Lemma (requires (add_set_key itsl k `contains` be))
+        (ensures (key_of be = k))
+
+(* get the blum evict element from an index *)
+val blum_evict_elem (#vcfg:_) (itsl: its_log vcfg) (i:I.seq_index itsl{is_evict_to_blum (I.index itsl i)}):
+  ms_hashfn_dom
+
+(* sequence of evicts in time sequence log *)
+val evict_seq (#vcfg:_) (itsl: its_log vcfg): seq ms_hashfn_dom
+
+(* set of evicts in time sequence log *)
+let evict_set #vcfg (itsl: its_log vcfg): mset_ms_hashfn_dom = 
+  seq2mset #_ #ms_hashfn_dom_cmp (evict_seq itsl)
+
+(* the evict sequence restricted to key k *)
+val evict_seq_key (#vcfg:_) (itsl: its_log vcfg) (k:key): seq ms_hashfn_dom
+
+let evict_set_key #vcfg (itsl: its_log vcfg) (k:key): mset_ms_hashfn_dom= 
+  seq2mset #_ #ms_hashfn_dom_cmp (evict_seq_key itsl k)
+
+(* the blum evicts in time sequenced log should be the same as global evict set *)
+val evict_set_correct (#vcfg:_) (itsl: its_log vcfg):
+  Lemma (evict_set itsl == IntG.evict_set (g_logS_of itsl))
+
+
+val lemma_spec_rel_implies_same_add_seq (#vcfg:_) (ils: its_log vcfg{spec_rel ils})
+  : Lemma (ensures (let ilk = to_logk ils in 
+                    add_seq ils = SpecB.ts_add_seq ilk))
+          [SMTPat (spec_rel ils)]
